Intermediate work (everything is BROKEN)

GlobalSafety.v
@@ -18,7 +18,7 @@ Definition function_safety (f : function_ty) :=
 
 Definition program_safety (p : program_ty) : Prop :=
   forall fuel,
-    (run_program p fuel).(error) = false.
+    (fst (run_program_stream p fuel)).(error) = false.
 
 (* NOTE: This probably isn't a useful definition *)
 (*
@@ -41,6 +41,14 @@ Proof.
   - admit.
 Admitted.
 
+Theorem program_stream_maintains_error :
+  forall p fuel,
+    (fst (run_program_stream p fuel)).(error) = true ->
+    (fst (run_program_stream p (fuel + 1))).(error) = true.
+Proof.
+  admit.
+Admitted.
+
 Definition function_safety (f : function_ty) : Prop :=
   forall f cfg p n s fuel,
     well_formed_program p ->
@@ -58,7 +66,7 @@ Proof.
   admit.
 Admitted.
 
-(* NOTE: This probably isn't the correct forumlation *)
+(* NOTE: This probably isn't the correct formulation *)
 (*
 Theorem function_safety_implies_program_safety :
   forall p f,
@@ -70,9 +78,160 @@ Proof.
   unfold program_safety. intros. unfold run_program. unfold run_program'.
 *)
 
+(* Theorems TODO list:
+   - cf_check implies that indirect calls are safe
+   - program well-formedness implies getting the next instructions is safe
+*)
 
 
-Theorem function_safety_something :
+Theorem well_formed_find_edge_ret :
+  forall cfg n p f ,
+    well_formed_program p ->
+    In f p.(fun_list) ->
+    cfg = fst f ->
+    In n cfg.(nodes) ->
+    (last (fst n) Ret) = Ret ->
+    forall b,
+      find_edge cfg n b = None.
+Proof.
+  admit.
+Admitted.
+
+Theorem well_formed_find_edge_branch :
+  forall cfg n p f c,
+    well_formed_program p ->
+    In f p.(fun_list) ->
+    cfg = fst f ->
+    In n cfg.(nodes) ->
+    (last (fst n) Ret) = Branch c ->
+    exists n' n'',
+      find_edge cfg n True_Branch = Some n' /\
+      find_edge cfg n False_Branch = Some n'' /\
+      find_edge cfg n Non_Branch = None.
+Proof.
+  admit.
+Admitted.
+
+(* TODO: Might have to change how the conditional is handled *)
+Theorem well_formed_find_edge_non_branch :
+  forall cfg n p f c,
+    well_formed_program p ->
+    In f p.(fun_list) ->
+    cfg = fst f ->
+    In n cfg.(nodes) ->
+      (last (fst n) Ret) <> Ret ->
+      (last (fst n) Ret) <> Branch c ->
+      exists n',
+        find_edge cfg n True_Branch = None /\
+        find_edge cfg n False_Branch = None /\
+        find_edge cfg n Non_Branch = Some n'.
+Proof.
+  admit.
+Admitted.
+
+Theorem verified_function_lookup :
+  forall p,
+    well_formed_program p ->
+    verify_program p = true ->
+    forall s istream fuel r hd_i,
+      (s, istream) = run_program_stream p fuel ->
+      s.(error) = false ->
+      Some hd_i = hd_error istream ->
+      hd_i.(instr) = Indirect_Call r ->
+      (fst (run_program_stream p (fuel + 1))).(error) = false.
+Proof.
+  admit.
+Admitted.
+
+(* NOTE: shouldn't even need to run the verifier for this one, just well-formedness *)
+Theorem verified_function_call :
+  forall p,
+    well_formed_program p ->
+    forall s istream fuel hd_i f_name,
+      (s, istream) = run_program_stream p fuel ->
+      s.(error) = false ->
+      Some hd_i = hd_error istream ->
+      hd_i.(instr) = Direct_Call f_name ->
+      (fst (run_program_stream p (fuel + 1))).(error) = false.
+Proof.
+  admit.
+Admitted.
+
+Theorem verify_get_instrs_till_terminal :
+  forall cfg n fuel p f,
+    well_formed_program p ->
+    In f p.(fun_list) ->
+    cfg = fst f ->
+    In n cfg.(nodes) ->
+    snd (get_instrs_till_terminal cfg n fuel) <> error_return.
+Proof.
+  intros. unfold get_instrs_till_terminal.
+  induction fuel. unfold snd. discriminate.
+  fold get_instrs_till_terminal. fold get_instrs_till_terminal in IHfuel.
+  assert ((fst n) <> nil). unfold well_formed_program in H. destruct H. destruct H3. destruct H4. destruct H5.
+  - specialize H6 with f. apply H6 in H0. unfold well_formed_fun in H0. unfold well_formed_cfg in H0.
+    destruct H0. destruct H7. destruct H8. unfold non_empty_nodes in H8. specialize H8 with n. symmetry in H1.
+    rewrite H1 in H8. apply H8. apply H2.
+  - admit.
+    (* case (last (fst n) Ret); intros. *)
+Admitted.
+
+Theorem verify_get_next_instrs :
+  forall p cfg n i s fuel,
+    well_formed_program p ->
+    exists f,
+      In f p.(fun_list) ->
+      cfg = fst f ->
+      In n cfg.(nodes) ->
+      In i (fst n) ->
+      verify_program p = true ->
+      snd (get_next_instrs p cfg n i s fuel) <> error_return.
+Proof.
+  admit.
+Admitted.
+
+Theorem verified_program :
+  forall p,
+    well_formed_program p ->
+    verify_program p = true ->
+    program_safety p.
+Proof.
+  intros. unfold program_safety. intros. unfold run_program_stream.
+  pose proof verify_get_instrs_till_terminal as Hterminal.
+  specialize Hterminal with (fst (main p)) (start_node (fst (main p))) fuel p (main p).
+  assert (snd (get_instrs_till_terminal (fst (main p)) (start_node (fst (main p))) fuel) <> error_return).
+  apply Hterminal; auto.
+  unfold well_formed_program in H. destruct H. destruct H1. destruct H2. destruct H3. assumption.
+  unfold well_formed_program in H. destruct H. destruct H1. destruct H2. destruct H3.
+  specialize H4 with (main p). apply H4 in H3. unfold well_formed_fun in H3.
+  unfold well_formed_cfg in H3. destruct H3. destruct H5. destruct H6. assumption.
+
+  destruct (get_instrs_till_terminal (fst (main p)) (start_node (fst (main p))) fuel).
+  unfold snd in H1. case r. auto. admit.
+  unfold run_program_stream'. induction fuel.
+  simpl. reflexivity.
+  fold run_program_stream'. fold run_program_stream' in IHfuel.
+  simpl (error (start_state p)). simpl (exit (start_state p)). destruct (false || false)%bool. auto.
+  induction l. auto.
+  pose proof verify_get_instrs_till_terminal as Hterminal'.
+  pose proof verify_get_next_instrs as Hnext.
+  specialize Hnext with p (cfg a) (node a) (instr a) (run_instr p (instr a) (start_state p)) (S fuel).
+  destruct (get_next_instrs p (cfg a) (node a) (instr a) (run_instr p (instr a) (start_state p)) (S fuel)).
+  destruct r0.
+  - unfold run_instr. destruct (instr a); auto.
+    + destruct (function_lookup p (get_register (start_state p) r0)).
+      auto. admit.
+    + admit.
+  - admit.
+  - unfold run_program_stream'.
+
+
+  case (get_instrs_till_terminal (fst (main p)) (start_node (fst (main p))) fuel).
+  intros. case r. auto. admit.
+Admitted.
+
+
+Theorem function_safety_independent :
   forall p f n bb fun_name s fuel s' n',
     well_formed_program p ->
     verify_program p = true ->
@@ -88,6 +247,8 @@ Theorem function_safety_something :
 Proof.
 
 
+(* NOTE: old version *)
+(*
 Theorem verified_program :
   forall p,
     well_formed_program p ->
@@ -108,3 +269,4 @@ Proof.
     + simpl. reflexivity.
     + destruct (next_node (fst (main p)) (start_state p) (start_node (fst (main p)))).
       *
+*)
